QuickSortInLean/QuickSortPermutation.lean
@@ -3,33 +3,35 @@ import QuickSortInLean.QuickSort
 import QuickSortInLean.Induction
 
 theorem partitionImpl_permuted {α : Type} [Ord α]
-  {n : Nat} (arr : Vec α n) (first i j : Nat)
-  (fi : first ≤ i) (ij : i ≤ j) (jn : j < n) :
-  permuted n arr (partitionImpl arr first i j fi ij jn).2 := by
+  {n : Nat} (arr : Vec α n) (first i j last : Nat)
+  (fi : first ≤ i) (ij : i ≤ j) (jl : j ≤ last) (jn : j < n) :
+  permuted n first last arr (partitionImpl arr first i j fi ij jn).2 := by
   induction arr, first, i, j, fi, ij, jn using partitionImpl.induct with
   | base arr first i j fi ij jn =>
     simp [*]
     exact .refl
   | step_lt arr first i j fi ij jn _ _ _ _ _ _ ih =>
     simp [*]
-    exact ih
+    exact ih jl
   | step_ge arr first i j fi ij jn _ _ _ _ _ _ _ ih =>
     simp [*]
-    apply permuted.step ⟨i, by assumption⟩ ⟨j, jn⟩ ih
+    apply permuted.step ⟨i, by assumption⟩ ⟨j, jn⟩ fi ij jl (ih (Nat.le_trans (Nat.sub_le ..) jl))
 
 theorem partition_permuted {α : Type} [Ord α]
   {n : Nat} (arr : Vec α n) (first last : Nat)
   (fl : first ≤ last) (ln : last < n) :
-  permuted n arr (partition arr first last fl ln).2 := by
+  permuted n first last arr (partition arr first last fl ln).2 := by
   let result := partition arr first last fl ln
   let mid := result.1
   simp [partition, dbgTraceIfShared]
-  let p := partitionImpl_permuted arr first last last fl (Nat.le_refl _) ln
-  exact permuted.trans p (.step ⟨first, Nat.lt_of_le_of_lt fl ln⟩ ⟨mid, Nat.lt_of_le_of_lt mid.property.2 ln⟩ .refl)
+  let p := partitionImpl_permuted arr first last last last fl (Nat.le_refl _) (Nat.le_refl _) ln
+  exact permuted.trans p
+    (.step ⟨first, Nat.lt_of_le_of_lt fl ln⟩ ⟨mid, Nat.lt_of_le_of_lt mid.property.2 ln⟩
+      (Nat.le_of_eq (Eq.refl _)) mid.property.1 mid.property.2 .refl)
 
 theorem quickSortImpl_permuted {α : Type} [Ord α]
   {n : Nat} (arr : Vec α n) (first last : Nat) (ln : last < n) :
-  permuted n arr (quickSortImpl arr first last ln) := by
+  permuted n first last arr (quickSortImpl arr first last ln) := by
   induction arr, first, last, ln using quickSortImpl.induct with
   | base arr first last ln h =>
     simp [*]
@@ -38,10 +40,12 @@ theorem quickSortImpl_permuted {α : Type} [Ord α]
     simp [*]
     let p := partition_permuted arr first last (Nat.le_of_lt lt) ln
     rw [eq] at p
-    exact permuted.trans (permuted.trans p ih₁) ih₂
+    exact permuted.trans
+      (permuted.trans p (ih₁.cast_last (Nat.le_trans (Nat.sub_le ..) parted.1.property.2)))
+      (ih₂.cast_first (Nat.le_trans parted.1.property.1 (Nat.le_succ _)))
 
 theorem quickSort'_permuted  {α : Type} [Ord α] {n : Nat} (arr : Vec α n) :
-  permuted n arr (quickSort' arr) := by
+  permuted n 0 (n - 1) arr (quickSort' arr) := by
   simp [quickSort']
   match Nat.decLt 0 n with
   | isTrue h =>
